src/contracts_coq/return_to_sender.v
@@ -28,22 +28,16 @@ Require Import util.
 Import error.
 Require List.
 
-Section return_to_sender.
-
-
-
 Definition parameter_ty := unit.
 Definition storage_ty := unit.
 
-Context {get_contract_type : contract_constant -> error.M type} {env : @proto_env get_contract_type parameter_ty}.
+Module ContractContext <: syntax.ContractContext.
+  Axiom get_contract_type : contract_constant -> error.M type.
+  Definition self_type := parameter_ty.
+End ContractContext.
+Module semantics := Semantics ContractContext. Import semantics.
 
-Definition instruction := @syntax.instruction get_contract_type parameter_ty.
-Definition data := @semantics.data get_contract_type parameter_ty.
-Definition stack := @semantics.stack get_contract_type parameter_ty.
-Definition eval {A B : stack_type} := @semantics.eval _ _ env A B.
-Definition eval_precond := @semantics.eval_precond _ _ env.
-
-Definition return_to_sender : @full_contract get_contract_type parameter_ty storage_ty :=
+Definition return_to_sender : full_contract parameter_ty storage_ty :=
   (
     CDR ;;
     NIL operation ;;
@@ -135,5 +129,3 @@ Proof.
         -- congruence.
         -- discriminate.
 Qed.
-
-End return_to_sender.
